new file:   c/tlpi/exit_handler.c 	new file:   c/tlpi/fork_stdio_buf.c 	modified:   clojure/test_java_jdbc.clj 	new file:   coq/Lib/lib_list.glob 	new file:   coq/Lib/lib_list.v 	new file:   coq/Lib/lib_list.vo 	new file:   coq/Lib/lib_option.glob 	new file:   coq/Lib/lib_option.v 	new file:   coq/Lib/lib_option.vo 	new file:   coq/listn.v 	modified:   coq/regex.v 	modified:   coq/sort.v 	modified:   coq/test.v 	modified:   scm/evaluator/TODO

c/tlpi/fork_stdio_buf.c
@@ -1,0 +1,20 @@
+// ./a.out
+// ./a.out > log; cat log
+// very interesting, all to do with stdio buffer in user space
+
+
+#include "tlpi_hdr.h"
+
+int
+main(int argc, char *argv[])
+{
+  printf("Hello world\n");
+
+  write(STDOUT_FILENO, "Ciao\n", 5);
+
+  if (fork() == -1)
+    errExit("fork");
+
+  /* Both child and parent continue execution here */
+  exit(EXIT_SUCCESS);
+}
