coq/regex.v
@@ -23,11 +23,13 @@ of type Language r can easily be translated into a string via some
 
 Inductive Language : Exp -> Set := 
   | LangLit     : forall c:char, Language (Lit c)
-  | LangAnd     : forall r1 r2: Exp, Language(r1) -> Language(r2) -> Language(And r1 r2)
-  | LangOrLeft  : forall r1 r2: Exp, Language(r1) -> Language(Or r1 r2)
-  | LangOrRight : forall r1 r2: Exp, Language(r2) -> Language(Or r1 r2)
+  | LangAnd     : forall r1 r2: Exp, 
+                    Language r1  -> Language r2  -> Language (And r1 r2)
+  | LangOrLeft  : forall r1 r2: Exp, Language r1  -> Language (Or r1 r2)
+  | LangOrRight : forall r1 r2: Exp, Language r2  -> Language (Or r1 r2)
   | LangEmpty   : forall r: Exp, Language (Many r)
-  | LangMany    : forall r: Exp, Language (Many r) -> Language r -> Language (Many r).
+  | LangMany    : forall r: Exp, 
+                    Language (Many r) -> Language r -> Language (Many r).
 
 Fixpoint semantics {r:Exp}(s:Language r) : string :=
   match s with
@@ -39,20 +41,23 @@ Fixpoint semantics {r:Exp}(s:Language r) : string :=
     | LangMany r s1 s2    => semantics s1 ++ semantics s2
   end.
 
-(* We now attempt to formalize the relation 'recognize' which expresses the fact that
-a string is an element of the language defined by a regular expression. Since we have
-already formalized the notion of 'Language', the fact that s:string is 'recognized' by
-a regular expression r (i.e. that it belongs to its language), can be expressed as
-the fact that s = semantics x for some x:Language r. Rather than proceeding this way,
-we now attempt to define the 'recognize' relation directly as an inductive predicate.
-We shall then attempt to prove the equivalence between the two approaches. *)
+(* We now attempt to formalize the relation 'recognize' which expresses the 
+fact that a string is an element of the language defined by a regular expression. 
+Since we have already formalized the notion of 'Language', the fact that s:string 
+is 'recognized' by a regular expression r (i.e. that it belongs to its language), 
+can be expressed as the fact that s = semantics x for some x:Language r. Rather 
+than proceeding this way, we now attempt to define the 'recognize' relation 
+directly as an inductive predicate. We shall then attempt to prove the equivalence 
+between the two approaches. *)
 
 Inductive recognize : Exp -> string -> Prop :=
   | recogLit    : forall c:char, recognize (Lit c) (c::nil)
   | recogAnd    : forall (r1 r2:Exp)(s1 s2:string), 
       recognize r1 s1 -> recognize r2 s2 -> recognize (And r1 r2) (s1 ++ s2)
-  | recogOrLeft : forall (r1 r2:Exp)(s :string), recognize r1 s -> recognize (Or r1 r2) s
-  | recogOrRight: forall (r1 r2:Exp)(s :string), recognize r2 s -> recognize (Or r1 r2) s
+  | recogOrLeft : forall (r1 r2:Exp)(s :string), 
+      recognize r1 s -> recognize (Or r1 r2) s
+  | recogOrRight: forall (r1 r2:Exp)(s :string), 
+      recognize r2 s -> recognize (Or r1 r2) s
   | recogEmpty  : forall (r:Exp), recognize (Many r) nil
   | recogMany   : forall (r:Exp) (s1 s2: string), 
       recognize (Many r) s1 -> recognize r s2 -> recognize (Many r) (s1 ++ s2).
@@ -84,22 +89,112 @@ Proof.
   exact H2. exact H1.
 Qed.
 
+(* this definition is needed for the next lemma *)
+Definition Lang_of_Lit_Pred {r:Exp}(x:Language r) := (* major trick *)
+  match r (* return Language r -> Prop *) with
+   | Lit c => fun x => x = LangLit c
+   | other => fun _ => True
+ end x.
+ 
 Lemma Lang_of_Lit: forall (c:char)(x:Language (Lit c)),
   x = LangLit c.
 Proof.
-  intros c x.
+  intros c x. fold (Lang_of_Lit_Pred x).
+  cut(forall (r:Exp)(x:Language r), Lang_of_Lit_Pred x). eauto.
+  clear c x. intros r x. destruct x; simpl; auto.
+Qed.
+
+(* this definition is needed for the next lemma *)
+Definition Lang_of_And_Pred {r:Exp}(x:Language r) := (* major trick *)
+  match r with
+    | And r1 r2   => fun x => 
+        exists (x1: Language r1)(x2: Language r2), x = LangAnd r1 r2 x1 x2
+    | other       => fun _ => 
+        True
+  end x.
+
+Lemma Lang_of_And: forall (r1 r2: Exp)(x: Language (And r1 r2)),
+  exists (x1: Language r1)(x2: Language r2), 
+  x = LangAnd r1 r2 x1 x2.
+Proof. 
+  intros r1 r2 x. fold (Lang_of_And_Pred x).
+  cut(forall (r:Exp)(x:Language r), Lang_of_And_Pred x). eauto.
+  clear r1 r2 x. intros r x. destruct x; simpl; eauto.
+Qed.
+
+(* this definition is needed for the next lemma *)
+Definition Lang_of_Or_Pred {r:Exp}(x:Language r) := (* major trick *)
+  match r with
+    | Or r1 r2   => fun x => 
+        (exists (x1: Language r1), x = LangOrLeft r1 r2 x1) \/
+        (exists (x2: Language r2), x = LangOrRight r1 r2 x2)
+    | other       => fun _ => 
+        True
+  end x.
+
+Lemma Lang_of_Or: forall (r1 r2: Exp)(x: Language (Or r1 r2)),
+  (exists (x1: Language r1), x = LangOrLeft r1 r2 x1) \/
+  (exists (x2: Language r2), x = LangOrRight r1 r2 x2).
+Proof.
+  intros r1 r2 x. fold (Lang_of_Or_Pred x). 
+  cut(forall (r:Exp)(x:Language r), Lang_of_Or_Pred x). eauto.
+  clear r1 r2 x. intros r x. destruct x; simpl; eauto.
+Qed.
 
 
 
-(*
+(* this definition is needed for the next lemma *)
+Definition Lang_of_Many_Pred {r:Exp}(x:Language r) := (* major trick *)
+  match r with
+    | Many r'     => fun x => 
+        (x = LangEmpty r') \/
+        (exists (x1: Language (Many r'))(x2: Language r'), 
+          x = LangMany r' x1 x2)
+    | other       => fun _ => 
+        True
+  end x.
+
+
+Lemma Lang_of_Many: forall (r: Exp)(x: Language (Many r)),
+  (x = LangEmpty r) \/
+  (exists (x1: Language (Many r))(x2: Language r),
+    x = LangMany r x1 x2).
+Proof. 
+  intros r x. fold (Lang_of_Many_Pred x).
+  cut (forall (r: Exp)(x:Language r), Lang_of_Many_Pred x). eauto.
+  clear r x. intros r x. destruct x; simpl; eauto.
+Qed.
+
+
 Lemma in_language_imp_recognize: forall (r:Exp)(s:string),
   (exists x:Language r, semantics x = s) -> recognize r s. 
 Proof.
+  (* induction on r *)
   intro r. elim r. 
-  clear r. intros c s H.
-*)
+  (* Lit *)
+  clear r. intros c s H. elim H. intros x Hx. generalize (Lang_of_Lit c x).
+  intro Hx'. rewrite Hx' in Hx. simpl in Hx. rewrite <- Hx. apply recogLit.
+  (* And *)
+  clear r. intros r1 H1 r2 H2 s H. elim H. intros x Hx. clear H.
+  generalize (Lang_of_And r1 r2 x). intro H'. elim H'. intro x1. clear H'.
+  intro H'. elim H'. intro x2. clear H'. intro H'. rewrite H' in Hx.
+  simpl in Hx. set (s1:= semantics x1). set (s2:=semantics x2).
+  fold s1 in Hx. fold s2 in Hx. rewrite <- Hx. apply recogAnd.
+  apply H1. exists x1. reflexivity. apply H2. exists x2. reflexivity.
+  (* Or *)
+  clear r. intros r1 H1 r2 H2 s H. elim H. intros x Hx. clear H. 
+  generalize (Lang_of_Or r1 r2 x). intro H. elim H. 
+  clear H. intro Hleft. elim Hleft. intros x1 H. rewrite H in Hx. simpl in Hx.
+  apply recogOrLeft. apply H1. exists x1. exact Hx.
+  clear H. intro Hright. elim Hright. intros x2 H. rewrite H in Hx. simpl in Hx.
+  apply recogOrRight. apply H2. exists x2. exact Hx.
+  (* Many *)
+  clear r. intros r Hr s H. elim H. intros x Hx. clear H.
+  generalize (Lang_of_Many r x). intro H. elim H. 
+  clear H. intro H. rewrite H in Hx. simpl in Hx. rewrite <- Hx. apply recogEmpty.
+  clear H. intro H. elim H. clear H. intros x1 H. elim H. clear H. intros x2 H.
+  rewrite H in Hx. simpl in Hx. rewrite <- Hx. apply recogMany.
 
 
 
-
-    
+   
