coq/test.v
@@ -1,29 +1,5 @@
-Parameter A:Set.
-
-Inductive List : nat -> Set :=
-  | ListNil   : List 0
-  | ListCons  : forall (n:nat), A -> List n -> List (S n).
-
-
-Fixpoint semantics {n:nat}(l: List n) : list A :=
-  match l with
-    | ListNil           => nil
-    | ListCons n a l'   => (cons a (semantics l'))
-  end.
-
-Definition simple {n:nat}(l: List n) : nat :=
-  match l with
-    | ListNil         => 0
-    | ListCons n a l' => 1
-  end.
-
-Lemma onlyList0: forall x:List 0,
-  x = ListNil.
-Proof.
- intro x.
- pose (g:= fun (n:nat)(l: List n) => 
-        match l with
-          | ListNil         => ListNil
-          | ListCons n a l' => x
-        end).
-
+Definition bar (a:Type) := a->Type.
+(*
+Definition foo (a:Type)(b:bar a):= prod a b.
+*)
+Definition foo (a:Type) := prod a (bar a).
