coq/Lib/lib_list.v
@@ -1,0 +1,27 @@
+Require Import List.
+
+Lemma nil_or_not_nil : forall (A:Type)(l:list A),
+  l = nil \/ l <> nil.
+Proof.
+  intros A l. elim l. left. reflexivity. clear l.
+  intros a l. intros. right. unfold not. intros. discriminate.
+Qed.
+
+
+(* This lemma is part of the Coq 8.5 library *)
+Lemma length_zero_iff_nil : forall (A:Type) (l:list A),
+  length l = 0 <-> l = nil.
+Proof.
+  intros A l. elim l. unfold length. split; auto. 
+  clear l. intros a l H. split. clear H. simpl. intro H.
+  discriminate H. clear H. intro H. discriminate H.
+Qed.
+
+Lemma length_of_tl : forall (A:Type) (l: list A),
+  l <> nil -> S (length (tl l)) = length l.
+Proof.
+  intros A l. elim l. unfold not. intro H. apply False_ind. auto.
+  clear l. intros a l IH. intro H. clear H. simpl. reflexivity.
+Qed.
+
+
