coq/Lib/lib_option.v
@@ -1,0 +1,18 @@
+Lemma not_none_is_some : forall (A:Type) (o: option A),
+  o <> None <-> exists x:A, o = Some x.
+Proof.
+  intros A o. split. elim o. intros a H. exists a. reflexivity.
+  intro H. apply False_ind. apply H. reflexivity.
+  intro H. elim H. intros x Hx. rewrite Hx. intros. discriminate.
+Qed.
+
+Lemma none_or_not_none : forall (A:Type) (o:option A),
+  o = None \/ o <> None.
+Proof.
+  intros A o. elim o. intro a. right. intro H. discriminate.
+  left. reflexivity.
+Qed.
+
+
+
+
