coq/listn.v
@@ -1,0 +1,67 @@
+Parameter A:Set.
+
+Inductive List : nat -> Set :=
+  | ListNil   : List 0
+  | ListCons  : forall (n:nat), A -> List n -> List (S n).
+
+
+Definition Pred {n:nat}(l: List n) :=
+  match n (* return List n -> Prop *) with
+    | 0 => fun l => l = ListNil
+    | _ => fun _ => True
+  end l.
+
+Lemma general : forall {n:nat} (l:List n), Pred l.  
+Proof.
+  intros n l. unfold Pred. destruct l; auto.  
+Qed.
+
+
+
+
+(*
+fun (n : nat) (l : List n) =>
+match l as l0 in (List n0) return (Pred l0) with
+| ListNil => eq_refl
+| ListCons _ _ _ => I
+end
+*)
+
+Definition proof {n:nat}(l: List n) :=
+  match l as l0 in (List n0) return (Pred l0) with
+    | ListNil => eq_refl
+    | ListCons _ _ _ => I
+  end.
+
+
+Lemma onlyList0: forall x:List 0,
+  x = ListNil.
+Proof.
+  intro x. apply general with (l:=x).
+Qed.
+
+
+Lemma l0_gen (n:nat) (l: List n) :
+  match n with
+    | 0 => fun l => l = ListNil
+    | _ => fun _ => True
+  end l.
+Proof.
+  now destruct l.
+Qed.
+
+
+Require Coq.Vectors.Vector.
+
+Lemma l0_gen' A n (v : Vector.t A n) :
+  match n (* return Vector.t A n -> Prop *) with
+    | 0 => fun v => v = @Vector.nil A
+    | _ => fun _ => True
+  end v.
+Proof.
+  now destruct v.
+Qed.
+
+
+
+
